update parser proofs after changing strategy for detecting left recursion

parser/Parser.v
@@ -48,6 +48,16 @@ Module ParserFn (Import D : Defs.T).
                  -> bool -> cache -> step_result
   | StepError  : parse_error -> step_result.
 
+  Lemma push_invar_eqs :
+    forall pm ss o x suf suf' frs,
+      stack_pushes_from_keyset pm ss
+      -> ss = (SF o suf, frs)
+      -> suf = NT x :: suf'
+      -> stack_pushes_from_keyset pm (SF o (NT x :: suf'), frs).
+  Proof.
+    intros; subst; auto.
+  Qed.
+
   Definition step (pm : production_map)
                   (cm : closure_map)
                   (ps : prefix_stack)
@@ -58,7 +68,92 @@ Module ParserFn (Import D : Defs.T).
                   (ca : cache)
                   (hc : cache_stores_target_results pm cm ca)
                   (hk : stack_pushes_from_keyset pm ss) : step_result := 
-    match ps, ss with
+    match ps with
+    | (PF pre v, p_frs) =>
+      match ss as ss' return ss = ss' -> _ with
+      | (SF o suf, s_frs) =>
+        fun hss => 
+          match suf as suf' return suf = suf' -> _ with
+          (* no more symbols to process in current frame *)
+          | [] =>
+            fun _ => 
+              match p_frs, s_frs with
+              (* empty stacks --> terminate *)
+              | [], [] => 
+                match ts with
+                | [] =>
+                  match v with
+                  | [t] => StepAccept t
+                  | _   => StepError InvalidState
+                  end
+                | _ :: _ => StepReject "stack exhausted, tokens remain"
+                end
+              (* nonempty stacks --> return to caller frames *)
+              | PF pre_cr v_cr :: p_frs', SF o_cr suf_cr :: s_frs' =>
+                match suf_cr with
+                | []                => StepError InvalidState
+                | T _  :: _         => StepError InvalidState
+                | NT x :: suf_cr'   =>
+                  let ps' := (PF (NT x :: pre_cr) (Node x (rev v) :: v_cr), p_frs') in
+                  let ss' := (SF o_cr suf_cr', s_frs')                              in
+                  StepK ps' ss' ts (NtSet.remove x vi) un ca          
+                end
+              | _, _ => StepError InvalidState
+              end
+          (* terminal case --> consume a token *)
+          | T a :: suf' =>
+            fun _ => 
+              match ts with
+              | []             => StepReject "input exhausted"
+              | (a', l) :: ts' =>
+                if t_eq_dec a' a then
+                  let ps' := (PF (T a :: pre) (Leaf a l :: v), p_frs) in
+                  let ss' := (SF o suf', s_frs)                       in
+                  StepK ps' ss' ts' NtSet.empty un ca
+                else
+                  StepReject "token mismatch"
+              end
+          (* nonterminal case --> push a frame onto the stack *)
+          | NT x :: suf' =>
+            fun hsuf => 
+              if NtSet.mem x vi then
+                (* Unreachable for a left-recursive grammar *)
+                match NM.find x pm with
+                | Some _ => StepError (LeftRecursion x) 
+                | None   => StepReject "nonterminal not in grammar" 
+                end
+              else
+                match adaptivePredict pm cm o x suf' s_frs ts ca hc
+                                      (push_invar_eqs _ _ _ _ _ _ _ hk hss hsuf)
+                with
+                | (PredSucc rhs, ca') =>
+                  let ps' := (PF [] [], PF pre v :: p_frs)        in
+                  let ss' := (SF (Some x) rhs, SF o suf :: s_frs) in
+                  StepK ps' ss' ts (NtSet.add x vi) un ca'
+                | (PredAmbig rhs, ca') =>
+                  let ps' := (PF [] [], PF pre v :: p_frs)        in
+                  let ss' := (SF (Some x) rhs, SF o suf :: s_frs) in
+                  StepK ps' ss' ts (NtSet.add x vi) false ca'
+                | (PredReject, _)  =>
+                  StepReject "prediction found no viable right-hand sides"
+                | (PredError e, _) =>
+                  StepError (PredictionError e) 
+                end
+          end eq_refl
+      end eq_refl
+    end.
+  
+(*  Definition step (pm : production_map)
+                  (cm : closure_map)
+                  (ps : prefix_stack)
+                  (ss : suffix_stack)
+                  (ts : list token)
+                  (vi : NtSet.t)
+                  (un : bool) 
+                  (ca : cache)
+                  (hc : cache_stores_target_results pm cm ca)
+                  (hk : stack_pushes_from_keyset pm ss) : step_result := 
+    match ps as , ss as ps', ss' return ps, ss = ps', ss' with
     | (PF pre v, p_frs), (SF o suf, s_frs) =>
       match suf with
       (* no more symbols to process in current frame *)
@@ -123,245 +218,269 @@ Module ParserFn (Import D : Defs.T).
           end
       end
     end.
-  
+ *)
+
   Lemma step_StepAccept_facts :
-    forall g pm hc cm ps ss ts vi un ca t,
-      step g pm hc cm ps ss ts vi un ca = StepAccept t
+    forall pm cm ps ss ts vi un ca hc hk t,
+      step pm cm ps ss ts vi un ca hc hk = StepAccept t
       -> ts = []
          /\ exists o, ss = (SF o [], [])
          /\ exists pre,
              ps = (PF pre [t], []).
   Proof.
-    intros g pm hc cm ps ss ts vi un ca v hs.
+    intros pm cm ps ss ts vi un ca hc hk t hs.
     unfold step in hs; dms; tc.
     inv hs; eauto.
   Qed.
 
   Lemma step_LeftRecursion_facts :
-    forall g pm hc cm ps ss ts vi un ca x,
-      step g pm hc cm ps ss ts vi un ca = StepError (LeftRecursion x)
-      -> ~ NtSet.In x av
-         /\ NtSet.In x (allNts g)
-         /\ exists o suf frs,
-             ss = (SF o (NT x :: suf), frs).
+    forall pm cm ps ss ts vi un ca hc hk x,
+      step pm cm ps ss ts vi un ca hc hk = StepError (LeftRecursion x)
+      -> NtSet.In x vi
+         /\ (exists yss, NM.find x pm = Some yss)
+         /\ (exists o suf frs,
+             ss = (SF o (NT x :: suf), frs)).
   Proof.
-    intros g cm pm hc ps ss ts vi un ca x hs.
+    intros cm pm ps ss ts vi un ca hc hk x hs.
     unfold step in hs; repeat dmeq h; tc; inv hs; sis;
       repeat split; eauto.
-    - unfold not; intros hi; apply NF.mem_iff in hi; tc.
-    - apply NF.mem_iff; auto.
+    apply NF.mem_iff; auto.
   Qed.
 
   Lemma step_preserves_cache_invar :
-    forall g pm hc cm ps ps' ss ss' ts ts' vi av' un un' ca ca',
-      cache_stores_target_results g pm hc cm ca
-      -> step g pm hc cm ps ss ts vi un ca = StepK ps' ss' ts' av' un' ca'
-      -> cache_stores_target_results g pm hc cm ca'.
+    forall pm cm ps ps' ss ss' ts ts' vi vi' un un' ca ca' hc hk,
+      step pm cm ps ss ts vi un ca hc hk = StepK ps' ss' ts' vi' un' ca'
+      -> cache_stores_target_results pm cm ca'.
   Proof.
-    intros gr pm hpc cm ps ps' ss ss' ts ts' vi av' un un' ca ca' hc hs.
+    intros pm cm ps ps' ss ss' ts ts' vi vi' un un' ca ca' hc hk hs.
     unfold step in hs; dmeqs H; tc; inv hs; auto.
     - eapply adaptivePredict_succ_preserves_cache_invar;  eauto.
     - eapply adaptivePredict_ambig_preserves_cache_invar; eauto.
   Defined.
 
-  Definition meas (g  : grammar)
+  Lemma step_preserves_push_invar :
+    forall pm cm ps ps' ss ss' ts ts' vi vi' un un' ca ca' hc hk,
+      step pm cm ps ss ts vi un ca hc hk = StepK ps' ss' ts' vi' un' ca'
+      -> stack_pushes_from_keyset pm ss'.
+  Proof.
+    intros pm cm ps ps' ss ss' ts ts' vi vi' un un' ca ca' hc hk hs.
+    unfold step in hs; dmeqs H; tc; inv hs; eauto.
+    - eapply return_preserves_pushes_invar; eauto.
+    - eapply consume_preserves_pushes_invar; eauto.
+    - eapply push_preserves_pushes_invar; eauto.
+      eapply rhssFor_keySet.
+      eapply adaptivePredict_succ_in_rhssFor; eauto.
+    - eapply push_preserves_pushes_invar; eauto.
+      eapply rhssFor_keySet.
+      (* lemma *)
+      eapply llPredict_ambig_in_rhssFor; eauto.
+      eapply adaptivePredict_ambig_llPredict_ambig; eauto.
+  Qed.
+
+  Definition meas (pm : production_map)
                   (ss : suffix_stack)
                   (ts : list token)
-                  (av :  NtSet.t) : nat * nat * nat := 
-    let m := maxRhsLength g    in
-    let e := NtSet.cardinal vi in
+                  (vi :  NtSet.t) : nat * nat * nat := 
+    let m := maxRhsLength (grammarOf pm)                in
+    let e := NtSet.cardinal (NtSet.diff (keySet pm) vi) in
     (List.length ts, stackScore ss (1 + m) e, stackHeight ss).
 
   Lemma meas_lt_after_return :
-    forall g ce cr cr' o o_cr x suf frs ts av,
-      ce  = SF o []
+    forall pm ce cr cr' o o_cr x suf frs ts vi,
+      ce     = SF o []
       -> cr  = SF o_cr (NT x :: suf)
       -> cr' = SF o_cr suf
-      -> lex_nat_triple (meas g (cr', frs) ts (NtSet.add x av))
-                        (meas g (ce, cr :: frs) ts av).
+      -> stack_pushes_from_keyset pm (ce, cr :: frs)
+      -> lex_nat_triple (meas pm (cr', frs) ts (NtSet.remove x vi))
+                        (meas pm (ce, cr :: frs) ts vi).
   Proof.
-    intros; subst; unfold meas.
+    intros ? ? ? ? ? ? ? ? ? ? ? ? ? ? hs;
+      subst; unfold meas; inv hs.
     pose proof stackScore_le_after_return as hs.
     eapply le_lt_or_eq in hs; eauto.
     destruct hs as [hlt | heq].
     - apply triple_snd_lt; eauto. 
-    - rewrite heq. apply triple_thd_lt; auto. 
+    - rewrite heq; apply triple_thd_lt; auto.
   Defined.
 
   Lemma meas_lt_after_push :
-    forall g cr ce o o' x suf rhs frs ts av,
+    forall pm cr ce o o' x suf rhs frs ts vi,
       cr = SF o (NT x :: suf)
       -> ce = SF o' rhs
-      -> In (x, rhs) g 
-      -> NtSet.In x av
-      -> lex_nat_triple (meas g (ce, cr :: frs) ts (NtSet.remove x av))
-                        (meas g (cr, frs) ts av).
+      -> In (x, rhs) (grammarOf pm)
+      -> ~ NtSet.In x vi
+      -> lex_nat_triple (meas pm (ce, cr :: frs) ts (NtSet.add x vi))
+                        (meas pm (cr, frs) ts vi).
   Proof.
     intros; subst.
     apply triple_snd_lt.
     eapply stackScore_lt_after_push; eauto.
+    eapply grammarOf_keySet; eauto.
   Defined.
 
   Lemma step_meas_lt :
-    forall g pm hc cm ps ps' ss ss' ts ts' vi av' un un' ca ca',
-      cache_stores_target_results g pm hc cm ca
-      -> step g pm hc cm ps ss ts vi un ca = StepK ps' ss' ts' av' un' ca'
-      -> lex_nat_triple (meas g ss' ts' av') (meas g ss ts av).
+    forall pm cm ps ps' ss ss' ts ts' vi vi' un un' ca ca' hc hk,
+      step pm cm ps ss ts vi un ca hc hk = StepK ps' ss' ts' vi' un' ca'
+      -> lex_nat_triple (meas pm ss' ts' vi') (meas pm ss ts vi).
   Proof.
-    intros g pm hpc cm ps ps' ss ss' ts ts' vi av' un un' ca ca' hc hs; unfold step in hs.
+    intros pm cm ps ps' ss ss' ts ts' vi vi' un un' ca ca' hc hk hs; unfold step in hs.
     destruct ss as ([ o [| [a|x] suf] ], frs).
     - dms; tc; inv hs.
       eapply meas_lt_after_return; eauto.
     - dms; tc; inv hs.
       apply triple_fst_lt; auto.
     - destruct ps as ([pre v], p_frs).
-      destruct (NtSet.mem x av) eqn:hm; [.. | dms; tc].
-      apply NF.mem_iff in hm.
-      destruct (adaptivePredict _ _ _ _ _ _) eqn:hp; dms; tc; inv hs.
+      destruct (NtSet.mem x vi) eqn:hm; [dms; tc | ..].
+      apply NF.not_mem_iff in hm.
+      destruct (adaptivePredict _ _ _ _ _ _ _ _ _ _) eqn:ha; dms; tc; inv hs.
       + eapply meas_lt_after_push; eauto.
-        eapply adaptivePredict_succ_in_grammar; eauto.
+        apply rhssFor_grammarOf.
+        eapply adaptivePredict_succ_in_rhssFor; eauto.
       + eapply meas_lt_after_push; eauto.
-        eapply adaptivePredict_ambig_in_grammar; eauto.
+        apply rhssFor_grammarOf.
+        (* lemma *)
+        eapply llPredict_ambig_in_rhssFor.
+        eapply adaptivePredict_ambig_llPredict_ambig; eauto.
   Qed.
 
   Lemma StepK_result_acc :
-    forall g pm hc cm ps ps' ss ss' ts ts' vi av' un un' ca ca' (a : Acc lex_nat_triple (meas g ss ts av)),
-      cache_stores_target_results g pm hc cm ca
-      -> step g pm hc cm ps ss ts vi un ca = StepK ps' ss' ts' av' un' ca'
-      -> Acc lex_nat_triple (meas g ss' ts' av').
+    forall pm cm ps ps' ss ss' ts ts' vi vi' un un' ca ca'
+           hc hk (a : Acc lex_nat_triple (meas pm ss ts vi)),
+      step pm cm ps ss ts vi un ca hc hk = StepK ps' ss' ts' vi' un' ca'
+      -> Acc lex_nat_triple (meas pm ss' ts' vi').
   Proof.
     intros; eapply Acc_inv; eauto.
     eapply step_meas_lt; eauto.
   Defined.
   
-  Fixpoint multistep (gr : grammar)
-                     (pm : production_map)
-                     (hp : production_map_correct pm gr)
+  Fixpoint multistep (pm : production_map)
                      (cm : closure_map)
                      (ps : prefix_stack)
                      (ss : suffix_stack)
                      (ts : list token)
-                     (av : NtSet.t)
+                     (vi : NtSet.t)
                      (un : bool)
                      (ca : cache)
-                     (hc : cache_stores_target_results gr pm hp cm ca)
-                     (ha : Acc lex_nat_triple (meas gr ss ts av))
+                     (hc : cache_stores_target_results pm cm ca)
+                     (hk : stack_pushes_from_keyset pm ss)
+                     (ha : Acc lex_nat_triple (meas pm ss ts vi))
                      {struct ha} : parse_result :=
-    match step gr pm hp cm ps ss ts vi un ca as res return step gr pm hp cm ps ss ts vi un ca = res -> _ with
+    match step pm cm ps ss ts vi un ca hc hk as res return step pm cm ps ss ts vi un ca hc hk = res -> _ with
     | StepAccept v                  => fun _  => if un then Accept v else Ambig v
     | StepReject s                  => fun _  => Reject s
     | StepError e                   => fun _  => Error e
-    | StepK ps' ss' ts' av' un' ca' =>
-      fun hs => multistep gr pm hp cm ps' ss' ts' av' un' ca'
-                          (step_preserves_cache_invar _ _ _ _ _ _ _ _ _ _ _ _ _ _ _ _ hc hs)
-                          (StepK_result_acc _ _ _ _ _ _ _ _ _ _ _ _ _ _ _ _ ha hc hs)
+    | StepK ps' ss' ts' vi' un' ca' =>
+      fun hs => multistep pm cm ps' ss' ts' vi' un' ca'
+                          (step_preserves_cache_invar _ _ _ _ _ _ _ _ _ _ _ _ _ _ hc hk hs)
+                          (step_preserves_push_invar _ _ _ _ _ _ _ _ _ _ _ _ _ _ hc hk hs)
+                          (StepK_result_acc _ _ _ _ _ _ _ _ _ _ _ _ _ _ hc hk ha hs)
     end eq_refl.
 
   Lemma multistep_unfold :
-    forall gr pm hp cm ps ss ts vi un ca hc ha,
-      multistep gr pm hp cm ps ss ts vi un ca hc ha =
-      match step gr pm hp cm ps ss ts vi un ca as res return step gr pm hp cm ps ss ts vi un ca = res -> _ with
+    forall pm cm ps ss ts vi un ca hc hk ha,
+      multistep pm cm ps ss ts vi un ca hc hk ha =
+      match step pm cm ps ss ts vi un ca hc hk as res return step pm cm ps ss ts vi un ca hc hk = res -> _ with
       | StepAccept v                  => fun _  => if un then Accept v else Ambig v
       | StepReject s                  => fun _  => Reject s
       | StepError e                   => fun _  => Error e
-      | StepK ps' ss' ts' av' un' ca' =>
-        fun hs => multistep gr pm hp cm ps' ss' ts' av' un' ca'
-                            (step_preserves_cache_invar _ _ _ _ _ _ _ _ _ _ _ _ _ _ _ _ hc hs)
-                            (StepK_result_acc _ _ _ _ _ _ _ _ _ _ _ _ _ _ _ _ ha hc hs)
+      | StepK ps' ss' ts' vi' un' ca' =>
+        fun hs => multistep pm cm ps' ss' ts' vi' un' ca'
+                            (step_preserves_cache_invar _ _ _ _ _ _ _ _ _ _ _ _ _ _ hc hk hs)
+                            (step_preserves_push_invar _ _ _ _ _ _ _ _ _ _ _ _ _ _ hc hk hs)
+                            (StepK_result_acc _ _ _ _ _ _ _ _ _ _ _ _ _ _ hc hk ha hs)
       end eq_refl.
   Proof.
     intros; destruct ha; auto.
   Qed.
   
   Lemma multistep_cases' :
-    forall (gr  : grammar)
-           (pm  : production_map)
-           (hp  : production_map_correct pm gr)
+    forall (pm  : production_map)
            (cm  : closure_map)
            (ps  : prefix_stack)
            (ss  : suffix_stack)
            (ts  : list token)
-           (av  : NtSet.t)
+           (vi  : NtSet.t)
            (un  : bool)
            (ca  : cache)
-           (hc  : cache_stores_target_results gr pm hp cm ca)
-           (ha  : Acc lex_nat_triple (meas gr ss ts av))
+           (hc  : cache_stores_target_results pm cm ca)
+           (hk  : stack_pushes_from_keyset pm ss)
+           (ha  : Acc lex_nat_triple (meas pm ss ts vi))
            (sr  : step_result)
            (pr  : parse_result)
-           (heq : step gr pm hp cm ps ss ts vi un ca = sr),
-      match sr as res return (step gr pm hp cm ps ss ts vi un ca = res -> parse_result) with
+           (heq : step pm cm ps ss ts vi un ca hc hk = sr),
+      match sr as res return (step pm cm ps ss ts vi un ca hc hk = res -> parse_result) with
       | StepAccept sv                 => fun _ => if un then Accept sv else Ambig sv
       | StepReject s                  => fun _ => Reject s
       | StepError s                   => fun _ => Error s
-      | StepK ps' ss' ts' av' un' ca' =>
-        fun hs => multistep gr pm hp cm ps' ss' ts' av' un' ca'
-                            (step_preserves_cache_invar _ _ _ _ _ _ _ _ _ _ _ _ _ _ _ _ hc hs)
-                            (StepK_result_acc _ _ _ _ _ _ _ _ _ _ _ _ _ _ _ _ ha hc hs)
+      | StepK ps' ss' ts' vi' un' ca' =>
+        fun hs => multistep pm cm ps' ss' ts' vi' un' ca'
+                            (step_preserves_cache_invar _ _ _ _ _ _ _ _ _ _ _ _ _ _ hc hk hs)
+                            (step_preserves_push_invar _ _ _ _ _ _ _ _ _ _ _ _ _ _ hc hk hs)
+                            (StepK_result_acc _ _ _ _ _ _ _ _ _ _ _ _ _ _ hc hk ha hs)
       end heq = pr
       -> match pr with
          | Accept f => (sr = StepAccept f /\ un = true)
-                       \/ (exists ps' ss' ts' av' un' ca' hc' ha',
-                              sr = StepK ps' ss' ts' av' un' ca'
-                              /\ multistep gr pm hp cm ps' ss' ts' av' un' ca' hc' ha' = Accept f)
+                       \/ (exists ps' ss' ts' vi' un' ca' hc' hk' ha',
+                              sr = StepK ps' ss' ts' vi' un' ca'
+                              /\ multistep pm cm ps' ss' ts' vi' un' ca' hc' hk' ha' = Accept f)
          | Ambig f  => (sr = StepAccept f /\ un = false)
-                       \/ (exists ps' ss' ts' av' un' ca' hc' ha',
-                              sr = StepK ps' ss' ts' av' un' ca'
-                              /\ multistep gr pm hp cm ps' ss' ts' av' un' ca' hc' ha' = Ambig f)
+                       \/ (exists ps' ss' ts' vi' un' ca' hc' hk' ha',
+                              sr = StepK ps' ss' ts' vi' un' ca'
+                              /\ multistep pm cm ps' ss' ts' vi' un' ca' hc' hk' ha' = Ambig f)
          | Reject s => sr = StepReject s
-                       \/ (exists ps' ss' ts' av' un' ca' hc' ha',
-                              sr = StepK ps' ss' ts' av' un' ca'
-                              /\ multistep gr pm hp cm ps' ss' ts' av' un' ca' hc' ha' = Reject s)
+                       \/ (exists ps' ss' ts' vi' un' ca' hc' hk' ha',
+                              sr = StepK ps' ss' ts' vi' un' ca'
+                              /\ multistep pm cm ps' ss' ts' vi' un' ca' hc' hk' ha' = Reject s)
          | Error s  => sr = StepError s
-                       \/ (exists ps' ss' ts' av' un' ca' hc' ha',
-                              sr = StepK ps' ss' ts' av' un' ca'
-                              /\ multistep gr pm hp cm ps' ss' ts' av' un' ca' hc' ha' = Error s)
+                       \/ (exists ps' ss' ts' vi' un' ca' hc' hk' ha',
+                              sr = StepK ps' ss' ts' vi' un' ca'
+                              /\ multistep pm cm ps' ss' ts' vi' un' ca' hc' hk' ha' = Error s)
          end.
   Proof.
-    intros g pm hp cm ps ss ts vi un ca hc ha sr pr heq.
+    intros pm cm ps ss ts vi un ca hc hk ha sr pr heq.
     destruct pr; destruct sr; destruct un;
-      try solve [ intros; tc | intros h; inv h; auto | intros h; right; eauto 10].
+      try solve [ intros; tc | intros h; inv h; auto | intros h; right; eauto 12].
   Qed.
 
   Lemma multistep_cases :
-    forall (gr  : grammar)
-           (pm  : production_map)
-           (hp  : production_map_correct pm gr)
+    forall (pm  : production_map)
            (cm  : closure_map)
            (ps  : prefix_stack)
            (ss  : suffix_stack)
            (ts  : list token)
-           (av  : NtSet.t)
+           (vi  : NtSet.t)
            (un  : bool)
            (ca  : cache)
-           (hc  : cache_stores_target_results gr pm hp cm ca)
-           (ha  : Acc lex_nat_triple (meas gr ss ts av))
+           (hc  : cache_stores_target_results pm cm ca)
+           (hk  : stack_pushes_from_keyset pm ss)
+           (ha  : Acc lex_nat_triple (meas pm ss ts vi))
            (pr  : parse_result),
-      multistep gr pm hp cm ps ss ts vi un ca hc ha = pr
+      multistep pm cm ps ss ts vi un ca hc hk ha = pr
       -> match pr with
-         | Accept f => (step gr pm hp cm ps ss ts vi un ca = StepAccept f /\ un = true)
-                       \/ (exists ps' ss' ts' av' un' ca' hc' ha',
-                              step gr pm hp cm ps ss ts vi un ca = StepK ps' ss' ts' av' un' ca'
-                              /\ multistep gr pm hp cm ps' ss' ts' av' un' ca' hc' ha' = Accept f)
-         | Ambig f  => (step gr pm hp cm ps ss ts vi un ca = StepAccept f /\ un = false)
-                       \/ (exists ps' ss' ts' av' un' ca' hc' ha',
-                              step gr pm hp cm ps ss ts vi un ca = StepK ps' ss' ts' av' un' ca'
-                              /\ multistep gr pm hp cm ps' ss' ts' av' un' ca' hc' ha' = Ambig f)
-         | Reject s => step gr pm hp cm ps ss ts vi un ca = StepReject s
-                       \/ (exists ps' ss' ts' av' un' ca' hc' ha',
-                              step gr pm hp cm ps ss ts vi un ca = StepK ps' ss' ts' av' un' ca'
-                              /\ multistep gr pm hp cm ps' ss' ts' av' un' ca' hc' ha' = Reject s)
-         | Error s  => step gr pm hp cm ps ss ts vi un ca = StepError s
-                       \/ (exists ps' ss' ts' av' un' ca' hc' ha',
-                              step gr pm hp cm ps ss ts vi un ca = StepK ps' ss' ts' av' un' ca'
-                              /\ multistep gr pm hp cm ps' ss' ts' av' un' ca' hc' ha' = Error s)
+         | Accept f => (step pm cm ps ss ts vi un ca hc hk = StepAccept f /\ un = true)
+                       \/ (exists ps' ss' ts' vi' un' ca' hc' hk' ha',
+                              step pm cm ps ss ts vi un ca hc hk = StepK ps' ss' ts' vi' un' ca'
+                              /\ multistep pm cm ps' ss' ts' vi' un' ca' hc' hk' ha' = Accept f)
+         | Ambig f  => (step pm cm ps ss ts vi un ca hc hk = StepAccept f /\ un = false)
+                       \/ (exists ps' ss' ts' vi' un' ca' hc' hk' ha',
+                              step pm cm ps ss ts vi un ca hc hk = StepK ps' ss' ts' vi' un' ca'
+                              /\ multistep pm cm ps' ss' ts' vi' un' ca' hc' hk' ha' = Ambig f)
+         | Reject s => step pm cm ps ss ts vi un ca hc hk = StepReject s
+                       \/ (exists ps' ss' ts' vi' un' ca' hc' hk' ha',
+                              step pm cm ps ss ts vi un ca hc hk = StepK ps' ss' ts' vi' un' ca'
+                              /\ multistep pm cm ps' ss' ts' vi' un' ca' hc' hk' ha' = Reject s)
+         | Error s  => step pm cm ps ss ts vi un ca hc hk = StepError s
+                       \/ (exists ps' ss' ts' vi' un' ca' hc' hk' ha',
+                              step pm cm ps ss ts vi un ca hc hk = StepK ps' ss' ts' vi' un' ca'
+                              /\ multistep pm cm ps' ss' ts' vi' un' ca' hc' hk' ha' = Error s)
          end.
   Proof.
-    intros g pm hp cm ps ss ts vi un ca hc ha pr hm; subst.
+    intros pm cm ps ss ts vi un ca hc hk ha pr hm; subst.
     rewrite multistep_unfold.
     eapply multistep_cases'; eauto.
   Qed.
 
-  Lemma multistep_accept_cases :
+(*  Lemma multistep_accept_cases :
     forall (gr : grammar)
            (pm  : production_map)
            (hp  : production_map_correct pm gr)
@@ -377,9 +496,9 @@ Module ParserFn (Import D : Defs.T).
            (t  : tree),
       multistep gr pm hp cm ps ss ts vi un ca hc ha = Accept t
       -> (step gr pm hp cm ps ss ts vi un ca = StepAccept t /\ un = true)
-         \/ (exists ps' ss' ts' av' un' ca' hc' ha',
-                step gr pm hp cm ps ss ts vi un ca = StepK ps' ss' ts' av' un' ca'
-                /\ multistep gr pm hp cm ps' ss' ts' av' un' ca' hc' ha' = Accept t).
+         \/ (exists ps' ss' ts' vi' un' ca' hc' ha',
+                step gr pm hp cm ps ss ts vi un ca = StepK ps' ss' ts' vi' un' ca'
+                /\ multistep gr pm hp cm ps' ss' ts' vi' un' ca' hc' ha' = Accept t).
   Proof.
     intros ? ? ? ? ? ? ? ? ? ? ? ? ? hm; subst. 
     destruct (multistep_cases _ _ _ _ _ _ _ _ _ _ _ _ _ hm); auto.
@@ -401,9 +520,9 @@ Module ParserFn (Import D : Defs.T).
            (t  : tree),
       multistep gr pm hp cm ps ss ts vi un ca hc ha = Ambig t 
       -> (step gr pm hp cm ps ss ts vi un ca = StepAccept t /\ un = false)
-         \/ (exists ps' ss' ts' av' un' ca' hc' ha',
-                step gr pm hp cm ps ss ts vi un ca = StepK ps' ss' ts' av' un' ca'
-                /\ multistep gr pm hp cm ps' ss' ts' av' un' ca' hc' ha' = Ambig t).
+         \/ (exists ps' ss' ts' vi' un' ca' hc' ha',
+                step gr pm hp cm ps ss ts vi un ca = StepK ps' ss' ts' vi' un' ca'
+                /\ multistep gr pm hp cm ps' ss' ts' vi' un' ca' hc' ha' = Ambig t).
 
   Proof.
     intros ? ? ? ? ? ? ? ? ? ? ? ? ? hm; subst. 
@@ -426,9 +545,9 @@ Module ParserFn (Import D : Defs.T).
            (s  : string),
       multistep gr pm hp cm ps ss ts vi un ca hc ha = Reject s
       -> step gr pm hp cm ps ss ts vi un ca = StepReject s
-         \/ (exists ps' ss' ts' av' un' ca' hc' ha',
-                step gr pm hp cm ps ss ts vi un ca = StepK ps' ss' ts' av' un' ca'
-                /\ multistep gr pm hp cm ps' ss' ts' av' un' ca' hc' ha' = Reject s).
+         \/ (exists ps' ss' ts' vi' un' ca' hc' ha',
+                step gr pm hp cm ps ss ts vi un ca = StepK ps' ss' ts' vi' un' ca'
+                /\ multistep gr pm hp cm ps' ss' ts' vi' un' ca' hc' ha' = Reject s).
   Proof.
     intros ? ? ? ? ? ? ? ? ? ? ? ? ? hm; subst. 
     destruct (multistep_cases _ _ _ _ _ _ _ _ _ _ _ _ _ hm); auto.
@@ -449,9 +568,9 @@ Module ParserFn (Import D : Defs.T).
            (ha : Acc lex_nat_triple (meas gr ss ts av)),
       multistep gr pm hp cm ps ss ts vi un ca hc ha = Error InvalidState
       -> step gr pm hp cm ps ss ts vi un ca = StepError InvalidState
-         \/ (exists ps' ss' ts' av' un' ca' hc' ha',
-                step gr pm hp cm ps ss ts vi un ca = StepK ps' ss' ts' av' un' ca'
-                /\ multistep gr pm hp cm ps' ss' ts' av' un' ca' hc' ha' = Error InvalidState).
+         \/ (exists ps' ss' ts' vi' un' ca' hc' ha',
+                step gr pm hp cm ps ss ts vi un ca = StepK ps' ss' ts' vi' un' ca'
+                /\ multistep gr pm hp cm ps' ss' ts' vi' un' ca' hc' ha' = Error InvalidState).
   Proof.
     intros ? ? ? ? ? ? ? ? ? ? ? ? hm; subst.
     destruct (multistep_cases _ _ _ _ _ _ _ _ _ _ _ _ _ hm); auto.
@@ -473,9 +592,9 @@ Module ParserFn (Import D : Defs.T).
            (x  : nonterminal),
       multistep gr pm hp cm ps ss ts vi un ca hc ha = Error (LeftRecursion x)
       -> step gr pm hp cm ps ss ts vi un ca = StepError (LeftRecursion x)
-         \/ (exists ps' ss' ts' av' un' ca' hc' ha',
-                step gr pm hp cm ps ss ts vi un ca = StepK ps' ss' ts' av' un' ca'
-                /\ multistep gr pm hp cm ps' ss' ts' av' un' ca' hc' ha' = Error (LeftRecursion x)).
+         \/ (exists ps' ss' ts' vi' un' ca' hc' ha',
+                step gr pm hp cm ps ss ts vi un ca = StepK ps' ss' ts' vi' un' ca'
+                /\ multistep gr pm hp cm ps' ss' ts' vi' un' ca' hc' ha' = Error (LeftRecursion x)).
   Proof.
     intros ? ? ? ? ? ? ? ? ? ? ? ? ? hm; subst.
     destruct (multistep_cases _ _ _ _ _ _ _ _ _ _ _ _ _ hm); auto.
@@ -497,32 +616,41 @@ Module ParserFn (Import D : Defs.T).
            (e  : prediction_error),
       multistep gr pm hp cm ps ss ts vi un ca hc ha = Error (PredictionError e)
       -> step gr pm hp cm ps ss ts vi un ca = StepError (PredictionError e)
-         \/ (exists ps' ss' ts' av' un' ca' hc' ha',
-                step gr pm hp cm ps ss ts vi un ca = StepK ps' ss' ts' av' un' ca'
-                /\ multistep gr pm hp cm ps' ss' ts' av' un' ca' hc' ha' = Error (PredictionError e)).
+         \/ (exists ps' ss' ts' vi' un' ca' hc' ha',
+                step gr pm hp cm ps ss ts vi un ca = StepK ps' ss' ts' vi' un' ca'
+                /\ multistep gr pm hp cm ps' ss' ts' vi' un' ca' hc' ha' = Error (PredictionError e)).
   Proof.
     intros ? ? ? ? ? ? ? ? ? ? ? ? ? hm; subst.
     destruct (multistep_cases _ _ _ _ _ _ _ _ _ _ _ _ _ hm); auto.
   Qed.
-
-  Lemma empty_cache_stores_target_results :
-    forall gr pm hp cm,
-      cache_stores_target_results gr pm hp cm empty_cache.
+ *)
+  
+  Lemma cache_invar_starts_true :
+    forall pm cm,
+      cache_stores_target_results pm cm empty_cache.
   Proof.
-    intros gr pm hp cm sps a sps' hf.
+    intros pm cm sps a sps' hf.
     rewrite CacheFacts.empty_o in hf; tc.
   Defined.
+
+  Lemma push_invar_starts_true :
+    forall pm x,
+      stack_pushes_from_keyset pm (SF None [NT x], []).
+  Proof.
+    intros pm x; red; auto.
+  Qed.
 
   (* This curried pattern enables us to partially apply the parser to a grammar
      and compute the closure map once, instead of each time we parse an input *)
   Definition parse (g : grammar) : nonterminal -> list token -> parse_result :=
-    let pm := mkProductionMap g         in
-    let hp := mkProductionMap_correct g in
-    let cm := mkClosureMap g            in
+    let pm := mkProductionMap g in
+    let cm := mkClosureMap g    in
     fun (x : nonterminal) (ts : list token) =>
       let p_stk0 := (PF []   []    , []) in
       let s_stk0 := (SF None [NT x], []) in
-      multistep g pm hp cm p_stk0 s_stk0 ts (allNts g) true empty_cache
-                (empty_cache_stores_target_results g pm hp cm) (lex_nat_triple_wf _).
+      multistep pm cm p_stk0 s_stk0 ts NtSet.empty true empty_cache
+                (cache_invar_starts_true pm cm)
+                (push_invar_starts_true _ _)
+                (lex_nat_triple_wf _).
 
 End ParserFn.
